S2I/Definitions.v
@@ -1,0 +1,20 @@
+Require Import Source.CS.
+Require Import Source.PS.
+Require Import Intermediate.CS.
+Require Import Intermediate.PS.
+
+Module S.
+  Import Source.Language.
+  Import Source.CS.
+  Import Source.PS.
+  Module CS := CS.
+  Module PS := PS.
+End S.
+
+Module I.
+  Import Intermediate.Machine.
+  Import Intermediate.CS.
+  Import Intermediate.PS.
+  Module CS := CS.
+  Module PS := PS.
+End I.
