S2I/PartialForward.v
@@ -1,0 +1,517 @@
+Require Import Common.Definitions.
+Require Import Common.Memory.
+Require Import CompCert.Events.
+Require Import CompCert.Smallstep.
+Require Import CompCert.Behaviors.
+Require Import Source.Language.
+Require Import Source.GlobalEnv.
+Require Import Source.CS.
+Require Import Source.PS.
+Require Import Intermediate.Machine.
+Require Import Intermediate.PS.
+Require Import S2I.Compiler.
+Require Import S2I.Definitions.
+
+Section PartialForward.
+  Variable prog: Source.program.
+  Variable tprog: Intermediate.program.
+
+  Variable ctx: Program.interface.
+
+  Hypothesis input_program_well_formedness:
+    Source.well_formed_program prog.
+
+  Hypothesis input_program_closedness:
+    Source.closed_program prog.
+
+  Hypothesis context_validity:
+    forall C CI, PMap.MapsTo C CI ctx -> PMap.MapsTo C CI (Source.prog_interface prog).
+
+  Hypothesis successful_compilation:
+    compile_program prog = Some tprog.
+
+  (* we assume to have a forward simulation proved for whole programs
+     in the complete semantics (I.CS simulates S.CS) *)
+
+  Variable match_comp_mems: ComponentMemory.t -> ComponentMemory.t -> Prop.
+
+  Definition match_mems (mem1 mem2: Memory.t) : Prop :=
+    forall C Cmem Cmem',
+      PMap.MapsTo C Cmem mem1 /\ PMap.MapsTo C Cmem' mem2 ->
+      match_comp_mems Cmem Cmem'.
+
+  Variable match_stack_frames: Component.id * value * cont -> Pointer.t -> Prop.
+
+  Inductive match_stacks : list (Component.id * value * cont) -> list Pointer.t -> Prop :=
+  | match_stacks_nil:
+      match_stacks [] []
+  | match_stacks_cons: forall s1 s2 sf1 sf2,
+      match_stacks s1 s2 ->
+      match_stack_frames sf1 sf2 ->
+      match_stacks (sf1 :: s1) (sf2 :: s2).
+
+  Variable index: Type.
+  Variable order: index -> index -> Prop.
+
+  Hypothesis well_founded_order: well_founded order.
+
+  (* the matching relation is built on the previous definitions *)
+
+  Variable match_states : index -> S.CS.state -> I.CS.state -> Prop.
+
+  Hypothesis match_turn:
+    forall i scs ics psi,
+      match_states i scs ics  -> (turn_of ics psi <-> turn_of scs psi).
+
+  Hypothesis match_executing_component:
+    forall i gps mem1 regs pc C s mem2 k e,
+      match_states i (C, s, mem2, k, e) (gps, mem1, regs, pc) ->
+      Pointer.component pc = C.
+
+  Hypothesis match_related_stacks:
+    forall i gps mem1 regs pc C s mem2 k e,
+      match_states i (C, s, mem2, k, e) (gps, mem1, regs, pc) ->
+      match_stacks s gps.   
+
+  Hypothesis match_memories:
+    forall i gps mem1 regs pc C s mem2 k e,
+      match_states i (C, s, mem2, k, e) (gps, mem1, regs, pc) ->
+      match_mems mem1 mem2.
+
+  (* TODO this is a first attempt, think more about it *)
+  Hypothesis match_calls:
+    forall i gps mem1 regs pc C s mem2 k v C' P,
+      match_states i (C, s, mem1, Kcall C' P k, E_val (Int v)) (gps, mem2, regs, pc) ->
+      GlobalEnv.executing (GlobalEnv.init_genv tprog) pc (ICall C' P).
+
+  (* match_states is used to build the forward simulation *)
+
+  Hypothesis match_initial_states:
+    forall s1,
+      initial_state (S.CS.sem prog) s1 ->
+    exists i s2,
+      initial_state (I.CS.sem tprog) s2 /\ match_states i s1 s2.
+
+  Hypothesis match_final_states:
+    forall i s1 s2 r,
+      match_states i s1 s2 ->
+      final_state (S.CS.sem prog) s1 r ->
+      final_state (I.CS.sem tprog) s2 r.
+
+  Hypothesis simulation:
+    forall s1 t s1',
+      Step (S.CS.sem prog) s1 t s1' ->
+    forall i s2,
+      match_states i s1 s2 ->
+    exists i', exists s2',
+      (Plus (I.CS.sem tprog) s2 t s2' \/
+       Star (I.CS.sem tprog) s2 t s2' /\ order i' i) /\ match_states i' s1' s2'.
+
+  Theorem transl_program_correct:
+    forward_simulation (S.CS.sem prog) (I.CS.sem tprog).
+  Proof.
+    eapply Forward_simulation.
+    econstructor; eauto.
+  Qed.
+
+  (* global environments are built out of programs *)
+
+  Let SG : Source.GlobalEnv.global_env := Source.GlobalEnv.init_genv prog.
+  Let IG : Intermediate.GlobalEnv.global_env := Intermediate.GlobalEnv.init_genv tprog.
+
+  (* we assume to have a forward simulation from intermediate whole program to 
+     intermediate partial programs. This is what we usually call decomposition step *)
+
+  Hypothesis decomp_step_correct:
+    forall ics t ics',
+      I.CS.step IG ics t ics' ->
+    forall ips,
+      I.PS.partial_state ctx ics ips ->
+    exists ips',
+      I.PS.step ctx IG ips t ips' /\ I.PS.partial_state ctx ics' ips'.
+
+  Theorem decomp_star_E0:
+    forall ics ics' ips,
+      Star (I.CS.sem tprog) ics E0 ics' ->
+      I.PS.partial_state ctx ics ips ->
+    exists ips',
+      Star (I.PS.sem tprog ctx) ips E0 ips' /\
+      I.PS.partial_state ctx ics' ips'.
+  Proof.
+    intros.
+    assert (H' := H).
+    generalize dependent ips. induction H.
+    - intro. exists ips. split.
+      constructor. auto.
+    - intros.
+      destruct (decomp_step_correct s1 t1 s2 H ips H2) as [ips1 []].
+      specialize (IHstar H0 ips1 H4).
+      destruct IHstar as [ips' []].
+      exists ips'. split.
+      + eapply star_trans.
+        * eapply star_step. apply H3.
+          eapply star_refl. eauto.
+        * apply H5.
+        * rewrite E0_right. auto.
+      + assumption.
+  Qed.
+
+  Theorem decomp_plus_E0:
+    forall ics ics' ips,
+      Plus (I.CS.sem tprog) ics E0 ics' -> I.PS.partial_state ctx ics ips ->
+    exists ips',
+      Plus (I.PS.sem tprog ctx) ips E0 ips' /\ I.PS.partial_state ctx ics' ips'.
+  Proof.
+    intros.
+    inversion H; subst.
+    symmetry in H3.
+    destruct (Eapp_E0_inv t1 t2 H3); subst.
+    destruct (decomp_step_correct ics E0 s2 H1 ips H0) as [ips1 []].
+    destruct (decomp_star_E0 s2 ics' ips1 H2 H5) as [ips' []].
+    exists ips'. split.
+    - econstructor; eauto.
+    - auto.
+  Qed. 
+
+  Hypothesis decomp_initial_states:
+    forall ics,
+      I.CS.initial_state tprog ics ->
+    exists ips,
+      I.PS.initial_state tprog ctx ips /\ I.PS.partial_state ctx ics ips.
+
+  Hypothesis decomp_final_states:
+    forall ics ips r,
+      I.PS.partial_state ctx ics ips ->
+      I.CS.final_state IG ics r ->
+      I.PS.final_state tprog ctx ips r.
+
+  Theorem decomposition:
+    forward_simulation (I.CS.sem tprog) (I.PS.sem tprog ctx).
+  Proof.
+    eapply forward_simulation_step; eauto.
+  Qed.
+
+  Corollary decomposition_with_refinement:
+    forall beh1, program_behaves (I.CS.sem tprog) beh1 ->
+    exists beh2, program_behaves (I.PS.sem tprog ctx) beh2 /\ behavior_improves beh1 beh2.
+  Proof.
+    intros beh1 Hbeh1.
+    eapply forward_simulation_behavior_improves; eauto.
+    apply decomposition.
+  Qed.
+
+  (* we prove a forward simulation for partial programs *)
+  (* we start by defining the relation between partial states *)
+
+  Inductive match_stack_frames_p:
+    Component.id * option (value * CS.cont) -> I.PS.PartialPointer.t -> Prop :=
+  | match_stack_frames_without_holes: forall C b o v k,
+      match_stack_frames (C, v, k) (C, b, o) ->
+      match_stack_frames_p (C, Some (v, k)) (C, Some (b, o))
+  | match_stack_frames_with_holes: forall C,
+      match_stack_frames_p (C, None) (C, None).
+
+  Inductive match_stacks_p:
+    list (Component.id * option (value * CS.cont)) -> list I.PS.PartialPointer.t -> Prop :=
+  | match_stacks_nil_p:
+      match_stacks_p [] []
+  | match_stacks_cons_p: forall s1 s2 sf1 sf2,
+      match_stacks_p s1 s2 ->
+      match_stack_frames_p sf1 sf2 ->
+      match_stacks_p (sf1 :: s1) (sf2 :: s2).
+
+  Inductive match_states_p: index -> S.PS.state -> I.PS.state -> Prop :=
+  | match_states_program:
+      forall i scs ics sps ips,
+        match_states i scs ics ->
+        S.PS.partial_state ctx scs (S.PS.PC sps) ->
+        I.PS.partial_state ctx ics (I.PS.PC ips) ->
+        match_states_p i (S.PS.PC sps) (I.PS.PC ips)
+  | match_states_context:
+      forall i C1 C2 s1 s2 mem1 mem2 exec_st1 exec_st2,
+        C1 = C2 ->
+        match_stacks_p s1 s2 ->
+        match_mems mem1 mem2 ->
+        exec_st1 = exec_st2 ->
+        match_states_p i (S.PS.CC (C1, s1, mem1) exec_st1)
+                         (I.PS.CC (C2, s2, mem2) exec_st2).
+ 
+  (* now we prove the forwad simulation between partial semantics *)
+
+  Lemma transl_initial_states:
+    forall s1, S.PS.initial_state prog ctx s1 ->
+    exists i s2, I.PS.initial_state tprog ctx s2 /\
+            match_states_p i s1 s2.
+  Proof.
+  Admitted.
+
+  Lemma transl_final_states:
+    forall i (sps:S.PS.state) (ips:I.PS.state) (r:int),
+      match_states_p i sps ips ->
+      S.PS.final_state prog ctx sps r ->
+      I.PS.final_state tprog ctx ips r.
+  Proof.
+  Admitted.
+
+  (* this should be provable, although it might be quite technical *)
+  Lemma aux:
+    forall scs1 scs2 sps,
+      S.PS.partial_state ctx scs1 (S.PS.PC sps) ->
+      S.PS.partial_state ctx scs2 (S.PS.PC sps) ->
+    forall scs1' sps',
+      S.CS.kstep SG scs1 E0 scs1' ->
+      S.PS.partial_state ctx scs1' (S.PS.PC sps') ->
+    exists scs2',
+      S.CS.kstep SG scs2 E0 scs2' /\
+      S.PS.partial_state ctx scs2' (S.PS.PC sps').
+  Proof. Admitted.
+
+  Theorem transl_step_correct:
+    forall s1 t s1',
+      S.PS.kstep ctx SG s1 t s1' ->
+    forall i s2,
+      match_states_p i s1 s2 ->
+    exists i', exists s2',
+      (Plus (I.PS.sem tprog ctx) s2 t s2' \/
+       Star (I.PS.sem tprog ctx) s2 t s2' /\ order i' i) /\ match_states_p i' s1' s2'.
+  Proof.
+    intros s1 t s1' Hstep i s2 Hmatch.
+    inversion Hstep
+      as [ scs2 scs2' sps sps'
+           Hscs2_partial Hsource_step
+           Hscs2'_partial
+         | ?|?|?|?|?|?|?|?|?|?]; subst;
+    inversion Hmatch
+      as [ i' scs1 ics ? ips Hwmatch
+           Hscs1_partial Hics_partial |]; subst.
+
+    (** program has control **)
+
+    (* epsilon *)
+    - destruct (aux scs2 scs1 sps
+                    Hscs2_partial Hscs1_partial
+                    scs2' sps' Hsource_step Hscs2'_partial)
+        as [scs1' [Hsource_step' Hmatch']].
+      destruct (simulation
+                  scs1 E0 scs1' Hsource_step' i ics Hwmatch)
+        as [i'' [ics' [Hinter_step Hwmatch']]].
+      destruct ics' as [[[gps' mem'] regs'] pc'].
+      destruct Hinter_step.
+      + eapply decomp_plus_E0 in H; eauto.
+        destruct H as [ips' []].
+        eexists. exists ips'. split.
+        * left. auto.
+        * inversion H0; subst; subst ps.
+          ** econstructor; eauto.
+          ** (* contra *)
+             inversion Hmatch'; subst ps; subst.
+             unfold I.PS.is_context_component, turn_of, I.PS.state_turn in *.
+             unfold S.PS.is_program_component, S.PS.is_context_component in *.
+             unfold turn_of, S.PS.state_turn in *.
+             apply match_executing_component in Hwmatch'.
+             rewrite Hwmatch' in H6. contradiction.
+          ** (* contra *)
+             inversion Hmatch'; subst ps; subst.
+             unfold I.PS.is_context_component, turn_of, I.PS.state_turn in *.
+             unfold S.PS.is_program_component, S.PS.is_context_component in *.
+             unfold turn_of, S.PS.state_turn in *.
+             apply match_executing_component in Hwmatch'.
+             rewrite Hwmatch' in H6. contradiction.
+      + destruct H.
+        eapply decomp_star_E0 in H; eauto.
+        destruct H as [ips' []].
+        eexists i''. exists ips'. split.
+        * right. split. eauto. eauto.
+        * inversion H1; subst; subst ps.
+          ** econstructor; eauto.
+          ** (* contra *)
+             inversion Hmatch'; subst ps; subst.
+             unfold I.PS.is_context_component, turn_of, I.PS.state_turn in *.
+             unfold S.PS.is_program_component, S.PS.is_context_component in *.
+             unfold turn_of, S.PS.state_turn in *.
+             apply match_executing_component in Hwmatch'.
+             rewrite Hwmatch' in H7. contradiction.
+          ** (* contra *)
+             inversion Hmatch'; subst ps; subst.
+             unfold I.PS.is_context_component, turn_of, I.PS.state_turn in *.
+             unfold S.PS.is_program_component, S.PS.is_context_component in *.
+             unfold turn_of, S.PS.state_turn in *.
+             apply match_executing_component in Hwmatch'.
+             rewrite Hwmatch' in H7. contradiction.
+
+    (* internal call *)
+    - eexists. eexists. split.
+      + left. econstructor.
+        * inversion Hics_partial; subst.
+          eapply I.PS.Program_Internal_Call; eauto.
+          ** admit.
+          ** admit.
+          ** admit.
+          ** admit.
+          ** admit.
+          ** admit.
+          ** admit.
+        * econstructor.
+        * admit.
+      + admit.
+
+    (* internal return *)
+    - eexists. eexists. split.
+      + left. econstructor.
+        * eapply I.PS.Program_Internal_Return; eauto.
+          ** admit.
+          ** admit.
+          ** admit.
+          ** admit.
+          ** admit.
+        * econstructor.
+        * admit.
+      + admit.
+
+    (* external call *)
+    - eexists.
+      destruct ips as [[[gps_ mem_] regs_] pc_].
+      exists (I.PS.CC (C', (Pointer.component pc_,
+                       Some (Pointer.block pc_, Pointer.offset (Pointer.inc pc_))) :: gps_,
+                  PMapExtra.filter (fun k _ => negb (PMap.mem k ctx)) mem_) Normal).
+      split.
+      + left. econstructor.
+        * unfold step. simpl.
+          eapply I.PS.Program_External_Call;
+            inversion Hscs1_partial; subst;
+            inversion Hics_partial; subst.
+          (* we executing a call instruction *)
+          ** eapply match_calls; eauto.
+          (* we are not calling ourself *)
+          ** admit.
+          (* we are calling an imported procedure *)
+          ** admit.
+          (* we are calling the context *)
+          ** subst ps4.
+             unfold I.PS.is_program_component, I.PS.is_context_component in *.
+             unfold turn_of, I.PS.state_turn in *.
+             (* something is wrong, redo with correct existential instances*)
+             admit.
+          ** (* the stack changes *) admit.
+          ** (* the call argument is in R_COM *) admit.
+          ** admit.
+          ** admit.
+          ** admit.
+        * admit.
+        * admit.
+      + admit.
+
+    (* external return *)
+    - eexists.
+      destruct ips as [[[gps_ mem_] regs_] pc_].
+      eexists.
+      split.
+      + left. econstructor.
+        * admit.
+        * econstructor.
+        * admit.
+      + admit.
+
+    (** context has control **)
+
+    (* epsilon *)
+    - eexists. eexists. split.
+      + left. econstructor.
+        * eapply I.PS.Context_Epsilon; eauto.
+        * econstructor.
+        * auto.
+      + econstructor; auto.
+
+    (* goes wrong *)
+    - eexists. eexists. split.
+      + left. econstructor.
+        * eapply I.PS.Context_GoesWrong; eauto.
+        * econstructor.
+        * auto.
+      + econstructor; auto.
+
+    (* internal call *)
+    - eexists. eexists. split.
+      + left. econstructor.
+        * eapply I.PS.Context_Internal_Call; eauto.
+          ** auto.
+        * econstructor.
+        * subst t0. rewrite E0_right. eauto.
+      + econstructor; auto.
+        * constructor; auto.
+          constructor.
+
+    (* internal return *)
+    - inversion H2; subst.
+      eexists. exists (I.PS.CC (C', s2, mem2) Normal). split.
+      + left. econstructor.
+        * eapply I.PS.Context_Internal_Return; eauto.
+          ** auto.
+          ** inversion H7. subst. reflexivity.
+        * econstructor.
+        * subst t0. simpl. auto.
+      + econstructor; eauto.
+
+    (* external calls/returns depend on the match_states relation *)
+
+    (* external call *)
+    - eexists. eexists. split.
+      + left. econstructor.
+        * eapply I.PS.Context_External_Call; eauto.
+          ** auto.
+          ** (* the call argument that is in RCOM is the same argument I used 
+                in the source call *)
+            admit.
+          ** (* the entrypoint I'm jumping to corresponds to the procedure
+                I was calling at the source *)
+            admit.
+        * econstructor.
+        * subst t0. reflexivity.
+      + econstructor.
+        * admit.
+        * admit.
+        * admit.
+
+    (* external return *)
+    - eexists. eexists. split.
+      + left. econstructor.
+        * eapply I.PS.Context_External_Return; eauto.
+          (* we are returning to the program *)
+          ** unfold I.PS.is_program_component, I.PS.is_context_component.
+             unfold S.PS.is_program_component, S.PS.is_context_component in *.
+             simpl in *. eapply H.
+          ** (* the call return value that is in RCOM is the same return value of 
+                the source call *)
+            admit.
+          ** (* the stack changes as at the source *)
+            inversion H3; subst.
+            inversion H8; subst. admit.
+        * econstructor.
+        * subst t0. reflexivity.
+      + econstructor.
+        * admit.
+        * admit.
+        * admit.
+  Admitted.
+
+  (* I simulates S, L1=I.PS.sem L2=S.PS.sem *)
+  Theorem transl_program_correct_p:
+    forward_simulation (S.PS.sem prog ctx) (I.PS.sem tprog ctx).
+  Proof.
+    eapply Forward_simulation.
+    econstructor.
+    - eauto.
+    - apply transl_initial_states.
+    - apply transl_final_states.
+    - apply transl_step_correct.
+  Qed.
+
+  Corollary behavior_refinement_p:
+    forall beh1, program_behaves (S.PS.sem prog ctx) beh1 ->
+    exists beh2, program_behaves (I.PS.sem tprog ctx) beh2 /\ behavior_improves beh1 beh2.
+  Proof.
+    intros beh1 Hbeh1.
+    eapply forward_simulation_behavior_improves; eauto.
+    apply transl_program_correct_p.
+  Qed.
+End PartialForward.
